src/lib/communication/DY.Lib.Communication.RequestResponse.fst
@@ -102,11 +102,27 @@ instance local_state_communication_layer_session (a:Type) {|config:comm_layer_re
 }
 
 [@@with_bytes bytes]
+type sender_authentication = 
+  | Authenticated
+  | Unauthenticated
+
+#push-options "--ifuel 1"
+%splice [ps_sender_authentication] (gen_parser (`sender_authentication))
+%splice [ps_sender_authentication_is_well_formed] (gen_is_well_formed_lemma (`sender_authentication))
+#pop-options
+
+val request_authenticated: #a:Type -> {|comm_layer_reqres_config a|} -> comm_meta_data a -> sender_authentication
+let request_authenticated #a #config req_meta_data =
+  match req_meta_data.client with
+  | None -> Unauthenticated
+  | Some _ -> Authenticated
+
+[@@with_bytes bytes]
 type communication_reqres_event (a:Type) {|config:comm_layer_reqres_config a|} =
-  | CommClientSendRequest: [@@@ with_parser #bytes ps_bool] authenticated:bool -> client:principal -> server:principal -> [@@@ with_parser #bytes config.reqres_ps_a] request:a -> key:bytes -> communication_reqres_event a
+  | CommClientSendRequest: [@@@ with_parser #bytes ps_sender_authentication] authenticated:sender_authentication -> client:principal -> server:principal -> [@@@ with_parser #bytes config.reqres_ps_a] request:a -> key:bytes -> communication_reqres_event a
   | CommServerReceiveRequest: [@@@ with_parser #bytes (ps_option ps_principal)] client:option principal -> server:principal -> [@@@ with_parser #bytes config.reqres_ps_a] request:a -> key:bytes -> communication_reqres_event a
   | CommServerSendResponse: [@@@ with_parser #bytes (ps_option ps_principal)] client:option principal -> server:principal -> [@@@ with_parser #bytes config.reqres_ps_a] request:a -> [@@@ with_parser #bytes config.reqres_ps_a] response:a -> key:bytes -> communication_reqres_event a
-  | CommClientReceiveResponse: [@@@ with_parser #bytes ps_bool] authenticated:bool -> client:principal -> server:principal -> [@@@ with_parser #bytes config.reqres_ps_a] request:a -> [@@@ with_parser #bytes config.reqres_ps_a] response:a -> key:bytes -> communication_reqres_event a
+  | CommClientReceiveResponse: client:principal -> [@@@ with_parser #bytes config.reqres_ps_a] response:a -> req_meta_data:comm_meta_data a -> communication_reqres_event a
 
 #push-options "--ifuel 1"
 %splice [ps_communication_reqres_event] (gen_parser (`communication_reqres_event))
@@ -121,81 +137,56 @@ instance event_communication_reqres_event (#a:Type) {|config:comm_layer_reqres_c
 
 (*** API ***)
 
-(**** Unauthenticated Request ****)
-
+#push-options "--ifuel 1"
 [@@ "opaque_to_smt"]
 val send_request:
   #a:Type0 -> {|comm_layer_reqres_config a|} ->
+  authenticated:sender_authentication ->
   communication_keys_sess_ids ->
   principal -> principal -> a ->
   traceful (option (timestamp & comm_meta_data a))
-let send_request #a #config comm_keys_ids client server request =
+let send_request #a #config authenticated comm_keys_ids client server request =
   let* key = mk_rand (AeadKey (comm_layer_aead_tag a) empty) (comm_label client server) 32 in
-  trigger_event client (CommClientSendRequest false client server request key <: communication_reqres_event a);*
+  trigger_event client (CommClientSendRequest authenticated client server request key <: communication_reqres_event a);*
   let payload_bytes:bytes = serialize a request in
   let* sid = new_session_id client in
   set_state client sid (ClientSendRequest {server; request; key} <: communication_states a);*
   let req_payload:comm_message_t = RequestMessage {request=payload_bytes; key} in
-  let*? msg_id = send_confidential #comm_message_t #(comm_layer_tag_core_config_reqres a) comm_keys_ids client server req_payload in
-  let req_meta_data:comm_meta_data a = {key; client=None; server; sid; request} in
-  return (Some (msg_id, req_meta_data))
+  match authenticated with
+  | Authenticated ->
+    let*? msg_id = send_confidential_authenticated #comm_message_t #(comm_layer_tag_core_config_reqres a) comm_keys_ids client server req_payload in
+    let req_meta_data:comm_meta_data a = {key; client=Some client; server; sid; request} in
+    return (Some (msg_id, req_meta_data))
+  | Unauthenticated ->
+    let*? msg_id = send_confidential #comm_message_t #(comm_layer_tag_core_config_reqres a) comm_keys_ids client server req_payload in
+    let req_meta_data:comm_meta_data a = {key; client=None; server; sid; request} in
+    return (Some (msg_id, req_meta_data))
+#pop-options
 
 [@@ "opaque_to_smt"]
 val receive_request:
   #a:Type -> {|comm_layer_reqres_config a|} ->
+  authenticated:sender_authentication ->
   communication_keys_sess_ids ->
   principal -> timestamp ->
   traceful (option (a & comm_meta_data a))
-let receive_request #a comm_keys_ids server msg_id =
-  let*? req_msg_t:comm_message_t = receive_confidential #comm_message_t #(comm_layer_tag_core_config_reqres a) comm_keys_ids server msg_id in
+let receive_request #a authenticated comm_keys_ids server msg_id =
+  let*? (req_msg_t, client):(comm_message_t & option principal) = if authenticated = Authenticated then
+    let*? cm = receive_confidential_authenticated #comm_message_t #(comm_layer_tag_core_config_reqres a) comm_keys_ids server msg_id in
+    return (Some (cm.payload, Some cm.sender))
+  else
+    let*? payload = receive_confidential #comm_message_t #(comm_layer_tag_core_config_reqres a) comm_keys_ids server msg_id in
+    return (Some (payload, None))
+  in
   guard_tr (RequestMessage? req_msg_t);*?
   let RequestMessage req_msg = req_msg_t in
   let*? request = return (parse a req_msg.request) in
-  trigger_event server (CommServerReceiveRequest None server request req_msg.key <: communication_reqres_event a);*
+  trigger_event server (CommServerReceiveRequest client server request req_msg.key <: communication_reqres_event a);*
   let* sid = new_session_id server in
-  set_state server sid (ServerReceiveRequest {client=None; request; key=req_msg.key} <: communication_states a);*
-  let req_meta_data:comm_meta_data a = {key=req_msg.key; client=None; server; sid; request} in
+  set_state server sid (ServerReceiveRequest {client; request; key=req_msg.key} <: communication_states a);*
+  let req_meta_data:comm_meta_data a = {key=req_msg.key; client; server; sid; request} in
   return (Some (request, req_meta_data))
 
-
-(**** Authenticated Request ****)
-
-[@@ "opaque_to_smt"]
-val send_request_authenticated:
-  #a:Type0 -> {|comm_layer_reqres_config a|} ->
-  communication_keys_sess_ids ->
-  principal -> principal -> a ->
-  traceful (option (timestamp & comm_meta_data a))
-let send_request_authenticated #a #config comm_keys_ids client server request =
-  let* key = mk_rand (AeadKey (comm_layer_aead_tag a) empty) (comm_label client server) 32 in
-  trigger_event client (CommClientSendRequest true client server request key <: communication_reqres_event a);*
-  let payload_bytes:bytes = serialize a request in
-  let* sid = new_session_id client in
-  set_state client sid (ClientSendRequest {server; request; key} <: communication_states a);*
-  let req_payload:comm_message_t = RequestMessage {request=payload_bytes; key} in
-  let*? msg_id = send_confidential_authenticated #comm_message_t #(comm_layer_tag_core_config_reqres a) comm_keys_ids client server req_payload in
-  let req_meta_data:comm_meta_data a = {key; client=Some client; server; sid; request} in
-  return (Some (msg_id, req_meta_data))
-
-[@@ "opaque_to_smt"]
-val receive_request_authenticated:
-  #a:Type -> {|comm_layer_reqres_config a|} ->
-  communication_keys_sess_ids ->
-  principal -> timestamp ->
-  traceful (option (a & comm_meta_data a))
-let receive_request_authenticated #a comm_keys_ids server msg_id =
-  let*? cm:communication_message comm_message_t = receive_confidential_authenticated #comm_message_t #(comm_layer_tag_core_config_reqres a) comm_keys_ids server msg_id in
-  guard_tr (RequestMessage? cm.payload);*?
-  let RequestMessage req_msg = cm.payload in
-  let*? request = return (parse a req_msg.request) in
-  trigger_event server (CommServerReceiveRequest (Some cm.sender) server request req_msg.key <: communication_reqres_event a);*
-  let* sid = new_session_id server in
-  set_state server sid (ServerReceiveRequest {client=Some cm.sender; request; key=req_msg.key} <: communication_states a);*
-  let req_meta_data:comm_meta_data a = {key=req_msg.key; client=Some cm.sender; server; sid; request} in
-  return (Some (request, req_meta_data))
-
-
-(*** Response Handling ***)
 
 [@@ "opaque_to_smt"]
 val mk_comm_layer_response_nonce: #a:Type -> {|comm_layer_reqres_config a|} -> comm_meta_data a -> usage -> traceful (option bytes)
@@ -270,7 +261,7 @@ let receive_response #a client req_meta_data msg_id =
     | None -> true
     | Some client' ->  client = client');*?
   set_state client req_meta_data.sid (ClientReceiveResponse {server=csr.server; response=payload; key=csr.key} <: communication_states a);*
-  trigger_event client (CommClientReceiveResponse (Some? req_meta_data.client) client csr.server req_meta_data.request payload csr.key <: communication_reqres_event a);*
+  trigger_event client (CommClientReceiveResponse client payload req_meta_data <: communication_reqres_event a);*
   return (Some (payload, req_meta_data))
 
 
